fix: include trait attrs in literal embedded types

case_studies/tests/src/lib.rs
@@ -14,7 +14,7 @@ mod trait_deps;
 
 mod statics;
 
-//mod vec_client;
+mod vec_client;
 mod mixed;
 mod closures;
 
